Theorem relating simulation and trace inclusion.

Simulation.thy
@@ -1,6 +1,6 @@
 theory Simulation
 
-imports Main LTS
+imports Main LTS List2
 
 begin
 section {* Relating LTSes: simulation *}
@@ -11,7 +11,8 @@ text {* We formalize the notion of simulation on LTSes. Classic definitions of s
 often consider a single LTS, and simulation is established between two states of the same
 LTS. Here, a simulation is a relation @{text "r"} between the states of one LTS
 and the states of another LTS such that any transition taken by the former can be simulated
-by the latter. 
+by the latter. The development presented in this section aims to achieve the final theorem
+that extends the simulation to full behavior, i.e. sequence of transitions runs.
 
 The relation between states is the basis of a relation between transitions:
 the source and destinations must be pairwise related, and the label shall coincide. This
@@ -24,8 +25,8 @@ text {* The former transition used to extend the notion of simulation to the set
 transitions of two LTSes @{text "l1"} and @{text "l2"}. This is specified in the function 
 @{text "sim_trans"}: *}
 
-definition sim_trans :: "'st rel \<Rightarrow> ('st, 'ev) LTS \<Rightarrow> ('st, 'ev) LTS \<Rightarrow> bool" where
-  "sim_trans r l l' \<equiv> 
+definition sim_lts_trans :: "'st rel \<Rightarrow> ('st, 'ev) LTS \<Rightarrow> ('st, 'ev) LTS \<Rightarrow> bool" where
+  "sim_lts_trans r l l' \<equiv> 
     \<forall> s s' . (s, s') \<in> r \<longrightarrow>
       (\<forall> t \<in> trans l . src t = s \<longrightarrow>
         (\<exists> t' \<in> trans l' . src t' = s' \<and> sim_transition r t t'))"
@@ -33,14 +34,14 @@ definition sim_trans :: "'st rel \<Rightarrow> ('st, 'ev) LTS \<Rightarrow> ('st
 text {* Another condition to establish a simulation between @{text "l"} and @{text "l'"}, is that 
 every initial state of the former must be related to an initial state of the latter by @{text "s"}: *}
 
-definition simulation_init :: "'st rel \<Rightarrow> ('st, 'ev) LTS \<Rightarrow> ('st, 'ev) LTS \<Rightarrow> bool" where
-  "simulation_init r l l' \<equiv> \<forall> s \<in> init l . \<exists> s' \<in> init l' . (s, s') \<in> r"
+definition sim_lts_init :: "'st rel \<Rightarrow> ('st, 'ev) LTS \<Rightarrow> ('st, 'ev) LTS \<Rightarrow> bool" where
+  "sim_lts_init r l l' \<equiv> \<forall> s \<in> init l . \<exists> s' \<in> init l' . (s, s') \<in> r"
 
 text {* We are now equiped to give the characterize that a relation @{text "r"} defines a simulation 
 of @{text "l"} by @{text "l'"}: *}
 
 definition simulation :: "'st rel \<Rightarrow> ('st, 'ev) LTS \<Rightarrow> ('st, 'ev) LTS \<Rightarrow> bool" where
-  "simulation r l l' \<equiv> simulation_init r l l' \<and> sim_trans r l l'"
+  "simulation r l l' \<equiv> sim_lts_init r l l' \<and> sim_lts_trans r l l'"
 
 text {* Based on the notion of simulation, we introduce the relation simulates on LTS: *}
 definition simulates :: "('st, 'ev) LTS \<Rightarrow> ('st, 'ev) LTS \<Rightarrow> bool" (infixl "\<sim>" 50) where
@@ -52,7 +53,7 @@ text {* Let us verify some basic properties of simulations. First we have that t
 identity relation establishes that a LTS simulates itself. *}
 
 lemma simulation_identity : "simulation Id l l" 
-  unfolding simulation_def simulation_init_def sim_trans_def sim_transition_def by auto
+  unfolding simulation_def sim_lts_init_def sim_lts_trans_def sim_transition_def by auto
 
 text {* Second, we have that the composition of two simulation relations is a simulation relation. *}
 lemma simulation_closed:
@@ -60,13 +61,13 @@ assumes s12: "simulation r12 l1 l2" and s23: "simulation r23 l2 l3"
 shows "simulation (r12 O r23) l1 l3"
 proof -
   from s12 s23
-  have "simulation_init (r12 O r23) l1 l3"
-  unfolding simulation_def simulation_init_def relcomp_unfold
+  have "sim_lts_init (r12 O r23) l1 l3"
+  unfolding simulation_def sim_lts_init_def relcomp_unfold
   by simp metis
 moreover
   from s12 s23
-  have "sim_trans (r12 O r23) l1 l3"
-  unfolding sim_trans_def simulation_def sim_transition_def relcomp_unfold
+  have "sim_lts_trans (r12 O r23) l1 l3"
+  unfolding sim_lts_trans_def simulation_def sim_transition_def relcomp_unfold
   by simp metis
   ultimately show ?thesis unfolding simulation_def ..
 qed
@@ -103,7 +104,7 @@ inductive sim_run :: "'st rel \<Rightarrow> ('st, 'ev) Run \<Rightarrow> ('st, '
 where
   "sim_run s [] []"
 | "sim_transition s t1 t2 \<Longrightarrow> sim_run s [t1] [t2]"
-| "ts1 \<noteq> [] \<and> ts2 \<noteq> [] \<and> sim_run s ts1 ts2 \<and> 
+| "ts1 \<noteq> [] \<and> sim_run s ts1 ts2 \<and> 
    sim_transition s t1 t2 \<and> dst t1 = src(hd ts1) \<and> dst t2 = src(hd ts2) \<Longrightarrow> 
    sim_run s (t1 # ts1) (t2 # ts2)"
 
@@ -111,30 +112,119 @@ text {* An important property on simulation and runs is that if a relation @{tex
 establishes a simulation of a run @{text "r"} with a run @{text "r'"}, then 
 @{text "r"} and @{text "r'"} are exhibit the same observable behavior: *}
 
-theorem "sim_run s r r' \<Longrightarrow> trace_of_run r = trace_of_run r'"
+theorem sim_run_trace_eq: "\<lbrakk>sim_run s r r'\<rbrakk> \<Longrightarrow> trace_of_run r = trace_of_run r'"
 proof(induct rule: sim_run.induct, simp, unfold sim_transition_def, simp, simp)
 qed
+
+text {* Lemma @{text "sim_run_empty_iff"} establishes that if there is a simulation
+between two runs, one run is empty if and only if the other run is also empty. *}
 
 lemma sim_run_empty_iff: "sim_run s r r' \<Longrightarrow> (r = [] \<longleftrightarrow> r' = [])"
 proof(induct rule: sim_run.induct, simp, simp, simp)
 qed
 
-lemma "sim_run s r r' \<and> r = [] \<Longrightarrow> r' = []"
-by (metis sim_run_empty_iff)
+text {* Lemma @{text "sim_run_all_trans"} gives that if there is a simulation @{text "s"}
+of run @{text "r"} by run @{text "r'"}, then @{text "s"} establishes a simulation of each
+transition of @{text "r"} with the corresponding transition of @{text "r'"}. *}
 
-lemma sim_run_last_trans: "sim_run s r r' \<Longrightarrow> r \<noteq> [] \<Longrightarrow> (dst(last r), dst(last r')) \<in> s"
-sorry
+lemma sim_run_all_trans: 
+  "\<lbrakk> sim_run s r r' \<rbrakk> \<Longrightarrow> List2.all (sim_transition s) r r'"
+proof(induct rule: sim_run.induct, auto)
+qed
+
+text {* The next lemma states that if \isasym{s} is a simulation between two non-empty runs,
+ then it is a simulation between the last states of these runs. *}
+ 
+lemma sim_run_last_trans: 
+  "\<lbrakk> sim_run s r r'; r \<noteq> [] \<rbrakk> \<Longrightarrow> sim_transition s (last r) (last r')"
+proof-
+  assume "sim_run s r r'" "r \<noteq> []"
+moreover
+  from `sim_run s r r'` and `r \<noteq> []` 
+    have "r' \<noteq> []" by (simp add: sim_run_empty_iff)
+moreover
+  from `sim_run s r r'` have "List2.all (sim_transition s) r r'" 
+    by (simp add: sim_run_all_trans)
+ultimately
+  show "(sim_transition s) (last r) (last r')" by (simp add: List2.last)
+qed
+
+text {* The next lemma states that if \isasym{s} is a simulation between two non-empty runs,
+ then the pair formed by the last states of the runs belongs to \isasym{s}. *}
+ 
+lemma sim_run_last_state: 
+  "\<lbrakk> sim_run s r r'; r \<noteq> [] \<rbrakk> \<Longrightarrow> (dst(last r), dst(last r')) \<in> s"
+proof-
+  assume "sim_run s r r'" "r \<noteq> []"
+  from `sim_run s r r'` and `r \<noteq> []` have "sim_transition s (last r) (last r')"
+    by (simp add: sim_run_last_trans)
+  then show ?thesis by (simp add:sim_transition_def)
+qed
+
+text {* Next, the following lemma establishes if \isasym{s} establishes a simulation between two 
+pairs of runs and the last state in the first pair coincides with the first state in the second run,
+then it also is a simulation between the concatenations of the runs. *}
+
+lemma sim_run_app_run: 
+  "\<lbrakk> sim_run (s :: 'st rel) (r1 :: ('st, 'ev) Run) (r1' :: ('st, 'ev) Run); 
+     sim_run s r2 r2'; r1 \<noteq> []; r2 \<noteq> []; dst(last r1) = src(hd r2); dst(last r1') = src(hd r2') \<rbrakk>
+   \<Longrightarrow> sim_run s (r1 @ r2) (r1' @ r2')"
+proof(induct rule: sim_run.induct, simp, simp)
+  fix s t1 t2
+  assume "sim_transition (s :: 'st rel) (t1 :: ('st, 'ev) Tr) (t2 :: ('st, 'ev) Tr)" 
+         "sim_run s r2 r2'" "r2 \<noteq> []" "dst t1 = src (hd r2)" "dst t2 = src (hd r2')"
+  then show "sim_run s (t1 # r2) (t2 # r2')" by(simp add:sim_run.intros(3))
+next
+  fix ts1 s ts2 t1 t2
+  assume hyp_induct: "ts1 \<noteq> [] \<and>
+       (sim_run s ts1 ts2 \<and>
+        (sim_run s r2 r2' \<longrightarrow>
+         ts1 \<noteq> [] \<longrightarrow> r2 \<noteq> [] \<longrightarrow> dst (last ts1) = src (hd r2) \<longrightarrow> dst (last ts2) = src (hd r2') 
+         \<longrightarrow> sim_run s (ts1 @ r2) (ts2 @ r2'))) \<and>
+       sim_transition s t1 t2 \<and> dst t1 = src (hd ts1) \<and> dst t2 = src (hd ts2)" 
+       "sim_run s r2 r2'" "r2 \<noteq> []"
+       "dst (last (t1 # ts1)) = src (hd r2)" "dst (last (t2 # ts2)) = src (hd r2')"
+  show "sim_run s ((t1 # ts1) @ r2) ((t2 # ts2) @ r2')"
+  proof-
+    from hyp_induct have "ts1 \<noteq> []" by simp
+  moreover
+    from hyp_induct have "sim_run s ts1 ts2" by simp
+    with `ts1 \<noteq> []` have "ts2 \<noteq> []" by (simp add:sim_run_empty_iff)
+    with hyp_induct have "dst (last ts2) = src (hd r2')" by simp
+    with `ts1 \<noteq> []` `sim_run s ts1 ts2` hyp_induct have "sim_run s (ts1 @ r2) (ts2 @ r2')" by simp
+  moreover
+    from hyp_induct have "sim_transition s t1 t2" by simp
+  moreover
+    from hyp_induct have "dst t1 = src (hd (ts1 @ r2))" by simp
+  moreover
+    from hyp_induct have "dst t2 = src (hd ts2)" by simp
+    with `ts2 \<noteq> []` have "dst t2 = src (hd (ts2 @ r2'))" by simp
+  ultimately
+    show "sim_run s ((t1 # ts1) @ r2) ((t2 # ts2) @ r2')" by (simp add:sim_run.intros)
+  qed
+qed
+
+text {* The following is a specialization of the latter lemma and establishes the property when
+exactly one transition is appended to two runs. *}
 
 lemma sim_run_app_trans: 
-  "sim_run s r r' \<Longrightarrow> r \<noteq> [] \<and> src t = dst(last r) \<and> src t' = dst(last r') \<and>
-  sim_transition s t t' \<Longrightarrow> sim_run s (r @ [t]) (r' @ [t'])"
-sorry
+  "\<lbrakk> sim_run s r r'; r \<noteq> []; src t = dst(last r); src t' = dst(last r'); sim_transition s t t'\<rbrakk> \<Longrightarrow> 
+  sim_run s (r @ [t]) (r' @ [t'])"
+proof-
+  assume "sim_run s r r'" "r \<noteq> []" "src t = dst(last r)" "src t' = dst(last r')" "sim_transition s t t'"
+moreover
+  from `sim_transition s t t'` have "sim_run s [t] [t']" by (simp add: sim_run.intros)
+moreover
+  from `sim_run s r r'` and `r \<noteq> []` have "r' \<noteq> []" by (simp add:sim_run_empty_iff)
+ultimately
+  show "sim_run s (r @ [t]) (r' @ [t'])" by (simp add:sim_run_app_run)
+qed
 
-text {* Next, we enunciate, and prove, the property that the existence of a simulation @{text "s"} 
-of the LTS @{text "l"} by the LTS @{text "l'"} guarantees that every run of the former may be 
+text {* Next, we present the an essential theorem, namely that a simulation @{text "s"} 
+of the LTS @{text "l"} by the LTS @{text "l'"} is also such that every run of the former may be 
 simulated with @{text "s"} by a run of the latter. *}
 
-lemma 
+theorem sim_run:
   assumes sim: "simulation s l l'" 
   shows "\<forall> r \<in> runs l . \<exists> r' \<in> runs l' . sim_run s r r'"
 proof
@@ -145,34 +235,51 @@ proof
     thus "\<exists> r' \<in> runs l'. sim_run s [] r'" by auto
   next
     fix t
-    assume step: "t \<in> trans l" and init: "src t \<in> init l"
-    with assms obtain s' where src: "(src t, s') \<in> s \<and> s' \<in> init l'" 
-      unfolding simulation_def simulation_init_def by blast
-    with step and assms obtain t' 
+    assume "t \<in> trans l" and "src t \<in> init l"
+    with assms obtain s' where s': "(src t, s') \<in> s \<and> s' \<in> init l'" 
+      unfolding simulation_def sim_lts_init_def by blast
+    with `t \<in> trans l` and assms obtain t' 
       where t': "t' \<in> trans l' \<and> src t' = s' \<and> sim_transition s t t'"
-      unfolding simulation_def sim_trans_def by blast
-    with src have "[t'] \<in> runs l'" by (metis runs.start)
-    with t' have "[t'] \<in> runs l' \<and> sim_run s [t] [t']" by (metis sim_run.intros(2))
-    hence "\<exists> r' . r' \<in> runs l' \<and> sim_run s [t] r'" ..
+      unfolding simulation_def sim_lts_trans_def by blast
+    with s' and t' have "[t'] \<in> runs l' \<and> sim_run s [t] [t']"
+      by (metis runs.start sim_run.intros(2))
     thus "\<exists> r' \<in> runs l'. sim_run s [t] r'" by auto
   next
     fix t r x
-    assume h0: "t \<in> trans l" and h1: "r \<noteq> []" and h2: "r \<in> runs l" and h3: "src t = dst (last r)" and
-    h4: "x \<in> runs l'" and h5: "sim_run s r x"
-    with sim have h6: "x \<noteq> []" by (metis sim_run_empty_iff)
-    from h1 and h5 have h7: "(dst(last r), dst(last x)) \<in> s" by (metis sim_run_last_trans)
-    obtain s' where h8: "s' = dst(last x)" by blast
-    from h7 and h8 have h9: "(dst(last r), s') \<in> s" by simp
-    from sim h0 h3 h9 obtain t' where t': "t' \<in> trans l' \<and> src t' = s' \<and> sim_transition s t t'" 
-      unfolding simulation_def sim_trans_def by blast
-    from t' h4 h6 and h8 have h10: "x @ [t'] \<in> runs l'" by (metis runs.step)
-    from h1 h5 h6 h3 h8 t' have h11: "sim_run s (r @ [t]) (x @ [t'])" by (metis sim_run_app_trans)
-    from h10 and h11 have "x @ [t'] \<in> runs l' \<and> sim_run s (r @ [t]) (x @ [t'])" ..
-    hence "\<exists> r' . r' \<in> runs l' \<and> sim_run s (r @ [t]) r'" ..
-    thus "\<exists> r' \<in> runs l'. sim_run s (r @ [t]) r'" by auto
+    assume 
+      "t \<in> trans l" and "r \<noteq> []" and "src t = dst (last r)" and
+      "x \<in> runs l'" and "sim_run s r x"
+    with sim have "x \<noteq> []" by (metis sim_run_empty_iff)
+    from `r \<noteq> []` and `sim_run s r x` 
+      have "(dst(last r), dst(last x)) \<in> s" by (metis sim_run_last_state)
+    with sim and `t \<in> trans l` and `src t = dst (last r)`
+      obtain t' where t': "t' \<in> trans l' \<and> src t' = dst(last x) \<and> sim_transition s t t'" 
+      unfolding simulation_def sim_lts_trans_def by (blast)
+    with `x \<in> runs l'` and `x \<noteq> []`
+      have "x @ [t'] \<in> runs l'" by (metis runs.step)
+  moreover
+    from `r \<noteq> []` and `sim_run s r x` and `src t = dst (last r)` and t' 
+      have "sim_run s (r @ [t]) (x @ [t'])" by (metis sim_run_app_trans)
+  ultimately
+    show "\<exists> r' \<in> runs l'. sim_run s (r @ [t]) r'" by auto
   qed
 qed
 
-end
+lemma sim_traces:
+  "\<lbrakk> simulation s l l' \<rbrakk> \<Longrightarrow> \<forall> t \<in> traces l . t \<in> traces l'"
+proof
+  fix t
+  assume "simulation s l l'" "t \<in> traces l"
+  from `t \<in> traces l` obtain r where "r \<in> runs l \<and> t = trace_of_run r" unfolding traces_def
+    by auto
+  with `simulation s l l'` obtain r' where "r' \<in> runs l' \<and> sim_run s r r'" 
+    by (metis sim_run)
+  with `r \<in> runs l \<and> t = trace_of_run r` have "t = trace_of_run r'" by (metis sim_run_trace_eq)
+  with `r' \<in> runs l' \<and> sim_run s r r'` show "t \<in> traces l'" unfolding traces_def by auto
+qed
 
+theorem sim_trace_inclusion: "\<lbrakk> simulation s l l' \<rbrakk> \<Longrightarrow> traces l \<subseteq> traces l'"
+by (metis sim_traces subsetI)
+
+end
 
